with old code

src/tactic/sort.lean
@@ -1,47 +1,207 @@
 import data.polynomial.degree.definitions
 import tactic
 
-open polynomial tactic
+namespace tactic
+
+/--  Given an expression `ei` and a list `l : list expr`, returns a `tactic expr` that is
+`ei + sum_of_list l`. -/
+meta def build_sum : expr → list expr → tactic expr
+| ei (e :: es) := do
+  e' ← build_sum ei es,
+  mk_app `has_add.add [e', e]
+| ei [] := pure ei
+
+/--  Takes an `expr` and returns a list of its summands. -/
+meta def get_summands : expr → list expr
+| `(%%a + %%b) := get_summands a ++ get_summands b
+| a            := [a]
+
+section with_weights
+variables {N : Type*} [has_lt N] [decidable_rel (has_lt.lt : N → N → Prop)]
+
+/--  Given an expression `a` and a weight function `wt : expr → N` to a Type `N` with `<`,
+`sort_summands_with_weight a wt` returns the list of summands appearing in `a`, sorted using the
+order `<`. -/
+meta def sort_summands_with_weight : expr → (expr → N) → list expr
+| a wt := (get_summands a).qsort (λ e f, wt e < wt f)
+
+/--  Let `wt : expr → N` be a "weight function": any function from `expr` to a Type `N` with a
+decidable relation `<`.
+
+Given an expression `e` in an additive commutative semigroup, `sorted_sum_with_weight wt e`
+returns an ordered sum of its terms, where the order is determined by applying `wt` to the summands
+appearing in `e`. -/
+meta def sorted_sum_with_weight (wt : expr → N) (e : expr) : tactic unit :=
+match sort_summands_with_weight e wt with
+| ei::es := do
+  el' ← build_sum ei es.reverse,
+  e_eq ← mk_app `eq [e, el'],
+  n ← get_unused_name,
+  assert n e_eq,
+  -- should we return a meaningful error if this does not manage to prove `e_eq`?
+  reflexivity <|> `[{ simp only [add_comm, add_assoc, add_left_comm], done, }],
+  h ← get_local n,
+  rewrite_target h,
+  clear h
+| [] := skip
+end
+
+/--  If the target is an equality, `sort_summands_lhs` sorts the summands on the lhs.
+-/
+meta def sort_summands_lhs (wt : expr → N) : tactic unit :=
+do
+  -- e ← get_local `h,
+  -- t ← infer_type e,
+  t ← target,
+  match t.is_eq with
+  | some (el, er) := do sorted_sum_with_weight wt el
+  | none          := trace "The goal is not an equality"
+  end
+
+/-- If the target is an equality, `sort_summands_rhs` sorts the summands on the rhs.
+-/
+meta def sort_summands_rhs (wt : expr → N) : tactic unit :=
+do
+  t ← target,
+  match t.is_eq with
+  | some (el, er) := do sorted_sum_with_weight wt er
+  | none          := trace "The goal is not an equality"
+  end
+
+/-- If the target is an equality, `sort_summands` sorts the summands on either side of the equality.
+-/
+meta def sort_summands (wt : expr → N) : tactic unit :=
+do
+  t ← target,
+  match t.is_eq with
+  | none          := fail "The goal is not an equality"
+  | some (el, er) := do
+    sorted_sum_with_weight wt el,
+    sorted_sum_with_weight wt er
+  end
+
+end with_weights
+
+/--  The order on `polynomial.monomial n r`, where monomials are compared by their "exponent" `n`.
+If the expression is not a monomial, then the weight is `⊥`. -/
+meta def monomial_weight : expr → with_bot ℕ
+| a := do
+  let as := match a.app_fn with
+  | `(coe_fn $ polynomial.monomial %%n) := n.to_nat
+  | _ := (⊥ : with_bot ℕ)  -- why do I have to remind Lean that this is `with_bot ℕ` and not `option ℕ`?
+  end,
+  as
+
+/--  If we have an expression involving monomials, `sum_sorted_monomials` returns an ordered sum
+of its terms.  Every summands that is not a monomial appears first, after that, monomials are
+sorted by increasing size of exponent. -/
+meta def sum_sorted_monomials (e : expr) : tactic unit :=
+sorted_sum_with_weight monomial_weight e
+
+/--  If the target is an equality involving monomials,
+then  `sort_monomials_lhs` sorts the summands on the lhs. -/
+meta def _root_.sort_monomials_lhs : tactic unit :=
+sort_summands_lhs monomial_weight
+
+/-- If the target is an equality involving monomials,
+then  `sort_monomials_rhs` sorts the summands on the rhs. -/
+meta def _root_.sort_monomials_rhs : tactic unit :=
+sort_summands_rhs monomial_weight
+
+/-- If the target is an equality involving monomials,
+then  `sort_monomials` sorts the summands on either side of the equality. -/
+meta def _root_.sort_monomials : tactic unit :=
+sort_summands monomial_weight
+
+end tactic
+
+open polynomial
 open_locale polynomial classical
 
-meta def is_sum : expr → bool
+variables {R : Type*} [semiring R] (f g : R[X]) {r s t u : R} (r0 : t ≠ 0)
+
+example :
+  (monomial 1) u + 5 * X +
+  (g + (monomial 5) 1) + ((monomial 0) s + (monomial 2) t + f) + (monomial 8) 1 =
+    X + monomial 7 1 + 2 * X :=
+begin
+  sort_monomials,
+  sort_monomials_lhs,
+  sort_monomials_rhs,
+  symmetry, sort_monomials_lhs
+end
+
+
+example : (X + f) * (X + f) = X * X + X * f + f * X + f * f :=
+begin
+  simp [add_mul, mul_add],
+  abel,
+end
+
+namespace tactic
+
+/--  Check whether an `expr` is a product of two terms. -/
+meta def is_mul : expr → bool
+| `(%%_ * %%_) := tt
+| _            := ff
+
+/--  Check whether an `expr` is a sum of two terms. -/
+meta def is_add : expr → bool
 | `(%%_ + %%_) := tt
 | _            := ff
 
-meta def get_monomials_from_sum_aux : expr → list (expr × option ℕ) → list (expr × option ℕ)
+/--  Check whether an `expr` is a `polynomial.monomial`. -/
+meta def is_monomial : expr → bool
+| `(coe_fn $ polynomial.monomial %%n) := tt
+| _            := ff
+
+/--  If `a : expr` is `monomial n r`, then `convert_monomial a = (a, (n : with_bot ℕ))`,
+otherwise `convert_monomial a = (a, ⊥)`. -/
+meta def convert_monomial : expr → expr × with_bot ℕ
+| a := do
+  let as := match a.app_fn with
+  | `(coe_fn $ polynomial.monomial %%n) := (a, expr.to_nat n)
+  | _ := (a, none)
+  end,
+  as
+
+meta def get_monomials_from_add_aux : expr → list (expr × with_bot ℕ) → list (expr × with_bot ℕ)
+| `(%%a + %%b) l := get_monomials_from_add_aux a l ++ get_monomials_from_add_aux b l
+| a l := convert_monomial a :: l
+
+meta def get_monomials_from_add_aux' : expr → list (expr × option ℕ) → list (expr × option ℕ)
 | `(%%a + %%b) l := do
   let as := match a.app_fn with
   | `(coe_fn $ polynomial.monomial %%n) := (a, expr.to_nat n) :: l
-  | _ := if (is_sum a) then get_monomials_from_sum_aux a l else (a, none) :: l
+  | _ := if (is_add a) then get_monomials_from_add_aux a l else (a, none) :: l
   end,
   let bs := match b.app_fn with
   | `(coe_fn $ polynomial.monomial %%n) := (b, expr.to_nat n) :: l
-  | _ := if (is_sum b) then get_monomials_from_sum_aux b l else (b, none) :: l
+  | _ := if (is_add b) then get_monomials_from_add_aux b l else (b, none) :: l
   end,
   as ++ bs
 | _ l := l
 
 meta def order_fn : expr × option ℕ → expr × option ℕ → bool
+| (_, none)    _          := tt
+| _           (_, none)   := ff
 | (_, some a) (_, some b) := a < b
-| (_, none) (_, some _) := tt
-| (_, some _) (_, none) := ff
-| _ _ := tt
 
-meta def get_sorted_monomials_from_sum (e : expr) : list expr :=
+meta def get_sorted_monomials_from_add (e : expr) : list expr :=
 do
-  let l := (get_monomials_from_sum_aux e []).qsort order_fn,
+  let l := (get_monomials_from_add_aux e []).qsort (λ x y, x.2 < y.2), --order_fn
   l.map (λ x, x.1)
 
-meta def build_sum : expr → list expr → tactic expr
+meta def build_add : expr → list expr → tactic expr
 | ei ((e : expr)::es) := do
-  e' ← build_sum ei es,
+  e' ← build_add ei es,
   mk_app `has_add.add [e', e]
 | ei [] := pure ei
 
-meta def sort_monomials_sum (e : expr) : tactic unit :=
-match get_sorted_monomials_from_sum e with
+meta def sort_monomials_add (e : expr) : tactic unit :=
+match get_sorted_monomials_from_add e with
 | ei::es := do
-  el' ← build_sum ei es.reverse,
+  el' ← build_add ei es.reverse,
   e_eq ← mk_app `eq [e, el'],
   n ← get_unused_name,
   assert n e_eq,
@@ -60,12 +220,12 @@ do
   match t.is_eq with
   | none          := fail "not an equality"
   | some (el, er) := do
-    sort_monomials_sum el,
-    sort_monomials_sum er
+    sort_monomials_add el,
+    sort_monomials_add er
   end
 
-example {R : Type*} [semiring R] {r s t u : R} (r0 : t ≠ 0) :
-  C u * X + X ^ 5 + C s + C t * X ^ 2 + X ^ 8 = 0 :=
+example {R : Type*} [semiring R] (f g : R[X]) {r s t u : R} (r0 : t ≠ 0) :
+  C u * X + (g + X ^ 5) + (C s + C t * X ^ 2 + f) + X ^ 8 = 0 :=
 begin
   try { unfold X },
   try { rw ← C_1 },
@@ -73,6 +233,9 @@ begin
   repeat { rw monomial_pow },
   repeat { rw monomial_mul_monomial },
   try { simp only [zero_add, add_zero, mul_one, one_mul, one_pow] },
-  sort_monomials, sort_monomials,
+  sort_monomials,
+  sort_monomials,
   -- ⇑(monomial 0) s + (⇑(monomial 1) u + (⇑(monomial 2) t + (⇑(monomial 5) 1 + ⇑(monomial 8) 1))) = 0
 end
+
+end tactic
